syntax: give SInstr a lightweight real semantics

syntax/SInstr.v
@@ -3,6 +3,8 @@ Require Import Bool.
 Require Import String.
 Require Import Ascii.
 Require Import ZArith.
+Require Import Lia.
+Require Import FunctionalExtensionality.
 Require Import StateTy.
 Require Import TyTy.
 Require Import InstrTy.
@@ -26,13 +28,20 @@ Module Ty <: TY.
 End Ty.
 
 Module State <: STATE.
-  Definition t := unit.
+  Definition t := MemCell -> Z.
   Definition non_alias (_ : t) := True.
-  Definition eq := @eq t.
-  Definition eq_refl := @eq_refl t.
-  Definition eq_trans := @eq_trans t.
-  Definition eq_sym := @eq_sym t.
-  Definition dummy_state := tt.
+  Definition eq (st1 st2 : t) : Prop := forall c, st1 c = st2 c.
+
+  Lemma eq_refl : forall s, eq s s.
+  Proof. intros s c. reflexivity. Qed.
+
+  Lemma eq_sym : forall s1 s2, eq s1 s2 -> eq s2 s1.
+  Proof. intros s1 s2 Heq c. symmetry. apply Heq. Qed.
+
+  Lemma eq_trans : forall s1 s2 s3, eq s1 s2 -> eq s2 s3 -> eq s1 s3.
+  Proof. intros s1 s2 s3 H12 H23 c. rewrite H12, H23. reflexivity. Qed.
+
+  Definition dummy_state : t := fun _ => 0%Z.
 End State.
 
 Module SInstr <: INSTR.
@@ -78,9 +87,6 @@ Module SInstr <: INSTR.
   Definition t := lang.
   Definition dummy_instr := SSkip.
 
-  Inductive sema : t -> list Z -> list MemCell -> list MemCell -> State.t -> State.t -> Prop := .
-  Definition instr_semantics := sema.
-
   Fixpoint affine_expr_eq_dec (e1 e2 : affine_expr) : {e1 = e2} + {e1 <> e2}.
   Proof. decide equality; try apply Z.eq_dec; try apply Nat.eq_dec. Defined.
 
@@ -115,25 +121,8 @@ Module SInstr <: INSTR.
   Qed.
 
   Definition NonAlias (_ : State.t) : Prop := True.
-
-  Lemma sema_prsv_nonalias :
-    forall i p wcs rcs st1 st2,
-      NonAlias st1 ->
-      instr_semantics i p wcs rcs st1 st2 ->
-      NonAlias st2.
-  Proof. intros; firstorder. Qed.
-
-  Lemma instr_semantics_stable_under_state_eq :
-    forall i p wcs rcs st1 st2 st1' st2',
-      State.eq st1 st1' ->
-      State.eq st2 st2' ->
-      instr_semantics i p wcs rcs st1 st2 ->
-      instr_semantics i p wcs rcs st1' st2'.
-  Proof. intros; firstorder. Qed.
-
   Definition InitEnv (env : list ident) (envv : list Z) (_ : State.t) : Prop :=
     length env = length envv.
-
   Definition Compat (_ : list (ident * Ty.t)) (_ : State.t) : Prop := True.
 
   Lemma init_env_samelen :
@@ -184,6 +173,186 @@ Module SInstr <: INSTR.
     | ExMul e1 e2 => read_accesses_expr e1 ++ read_accesses_expr e2
     end.
 
+  Definition normalize_affine (cols : nat) (aff : list Z * Z) : (list Z * Z) :=
+    let '(v, c) := aff in
+    (resize cols v, c).
+
+  Definition normalize_affine_list (cols : nat) (affs : list (list Z * Z)) :=
+    map (normalize_affine cols) affs.
+
+  Definition normalize_access (cols : nat) (acc : AccessFunction) : AccessFunction :=
+    let '(arrid, affs) := acc in
+    (arrid, normalize_affine_list cols affs).
+
+  Definition access_cols (acc : AccessFunction) : nat :=
+    let '(_, affs) := acc in
+    list_max (map (fun aff => let '(zs, _) := aff in length zs) affs).
+
+  Definition access_cell (a : access) (p : list Z) : MemCell :=
+    exact_cell (access_to_function a) p.
+
+  Definition memcell_eq_dec (c1 c2 : MemCell) : {cell_eq c1 c2} + {~ cell_eq c1 c2}.
+  Proof.
+    destruct c1 as [id1 idx1], c2 as [id2 idx2].
+    destruct (ident_eq_dec id1 id2) as [Hid|Hid].
+    - subst. destruct (veq_eq_dec idx1 idx2) as [Hidx|Hidx].
+      + left. split; auto.
+      + right. intros [Heq Hveq]. contradiction.
+    - right. intros [Heq _]. contradiction.
+  Defined.
+
+  Definition state_write (st : State.t) (cell : MemCell) (v : Z) : State.t :=
+    fun c => if memcell_eq_dec c cell then v else st c.
+
+  Fixpoint eval_expr (e : expr) (p : list Z) (st : State.t) : Z :=
+    match e with
+    | ExConst z => z
+    | ExVar n => nth n p 0%Z
+    | ExAccess a => st (access_cell a p)
+    | ExAdd e1 e2 => (eval_expr e1 p st + eval_expr e2 p st)%Z
+    | ExSub e1 e2 => (eval_expr e1 p st - eval_expr e2 p st)%Z
+    | ExMul e1 e2 => (eval_expr e1 p st * eval_expr e2 p st)%Z
+    end.
+
+  Fixpoint read_cells_expr (e : expr) (p : list Z) : list MemCell :=
+    match e with
+    | ExConst _ => []
+    | ExVar _ => []
+    | ExAccess a => [access_cell a p]
+    | ExAdd e1 e2 => read_cells_expr e1 p ++ read_cells_expr e2 p
+    | ExSub e1 e2 => read_cells_expr e1 p ++ read_cells_expr e2 p
+    | ExMul e1 e2 => read_cells_expr e1 p ++ read_cells_expr e2 p
+    end.
+
+  Inductive sema : t -> list Z -> list MemCell -> list MemCell -> State.t -> State.t -> Prop :=
+  | SemaSkip : forall p st1 st2,
+      State.eq st2 st1 ->
+      sema SSkip p [] [] st1 st2
+  | SemaAssign : forall lhs rhs p st1 st2 cell val,
+      cell = access_cell lhs p ->
+      val = eval_expr rhs p st1 ->
+      State.eq st2 (state_write st1 cell val) ->
+      sema (SAssign lhs rhs) p [cell] (read_cells_expr rhs p) st1 st2.
+
+  Definition instr_semantics := sema.
+
+  Lemma cell_eq_refl : forall c, cell_eq c c.
+  Proof. intros [id idx]; split; auto; apply veq_refl. Qed.
+
+  Lemma cell_eq_trans : forall c1 c2 c3, cell_eq c1 c2 -> cell_eq c2 c3 -> cell_eq c1 c3.
+  Proof.
+    intros [id1 idx1] [id2 idx2] [id3 idx3] [H12id H12idx] [H23id H23idx].
+    simpl in *. subst. split; [reflexivity|].
+    eapply veq_transitive; eauto.
+  Qed.
+
+  Lemma state_write_same : forall st cell v,
+    state_write st cell v cell = v.
+  Proof.
+    intros. unfold state_write.
+    destruct (memcell_eq_dec cell cell); [reflexivity|exfalso; apply n; apply cell_eq_refl].
+  Qed.
+
+  Lemma state_write_other : forall st cell1 cell2 v,
+    cell_neq cell2 cell1 ->
+    state_write st cell1 v cell2 = st cell2.
+  Proof.
+    intros. unfold state_write.
+    destruct (memcell_eq_dec cell2 cell1) as [Heq|Hneq]; [|reflexivity].
+    exfalso. destruct H as [Hid|Hidx]; destruct Heq as [Heqid Heqidx].
+    - exact (Hid Heqid).
+    - exact (Hidx Heqidx).
+  Qed.
+
+  Lemma state_write_proper : forall st1 st2 cell v,
+    State.eq st1 st2 ->
+    State.eq (state_write st1 cell v) (state_write st2 cell v).
+  Proof.
+    intros st1 st2 cell v Heq c. unfold state_write.
+    destruct (memcell_eq_dec c cell); auto.
+  Qed.
+
+  Lemma state_write_value_eq : forall st cell v1 v2,
+    v1 = v2 ->
+    State.eq (state_write st cell v1) (state_write st cell v2).
+  Proof.
+    intros st cell v1 v2 Heq c. unfold state_write.
+    destruct (memcell_eq_dec c cell); subst; reflexivity.
+  Qed.
+
+  Lemma state_write_commute : forall st cell1 cell2 v1 v2,
+    cell_neq cell1 cell2 ->
+    State.eq (state_write (state_write st cell1 v1) cell2 v2)
+             (state_write (state_write st cell2 v2) cell1 v1).
+  Proof.
+    intros st cell1 cell2 v1 v2 Hneq c.
+    unfold state_write.
+    destruct (memcell_eq_dec c cell2) as [Hc2|Hc2].
+    - destruct (memcell_eq_dec c cell1) as [Hc1|Hc1].
+      + exfalso.
+        destruct Hneq as [Hid|Hidx].
+        * destruct Hc1 as [Hid1 _]. destruct Hc2 as [Hid2 _].
+          apply Hid. transitivity (arr_id c); auto.
+        * destruct Hc1 as [_ Hidx1]. destruct Hc2 as [_ Hidx2].
+          apply Hidx. eapply veq_transitive; [apply veq_sym; exact Hidx1|exact Hidx2].
+      + reflexivity.
+    - destruct (memcell_eq_dec c cell1) as [Hc1|Hc1]; reflexivity.
+  Qed.
+
+  Lemma eval_expr_state_eq : forall e p st1 st2,
+    State.eq st1 st2 ->
+    eval_expr e p st1 = eval_expr e p st2.
+  Proof.
+    induction e; intros; simpl; try reflexivity.
+    - apply H.
+    - rewrite (IHe1 p st1 st2 H). rewrite (IHe2 p st1 st2 H). reflexivity.
+    - rewrite (IHe1 p st1 st2 H). rewrite (IHe2 p st1 st2 H). reflexivity.
+    - rewrite (IHe1 p st1 st2 H). rewrite (IHe2 p st1 st2 H). reflexivity.
+  Qed.
+
+  Lemma valid_access_cells_nil : forall p al,
+    valid_access_cells p [] al.
+  Proof.
+    unfold valid_access_cells. intros. contradiction.
+  Qed.
+
+  Lemma valid_access_cells_app : forall p c1 c2 al,
+    valid_access_cells p c1 al ->
+    valid_access_cells p c2 al ->
+    valid_access_cells p (c1 ++ c2) al.
+  Proof.
+    unfold valid_access_cells. intros p c1 c2 al H1 H2 c Hin.
+    apply in_app_or in Hin. destruct Hin; auto.
+  Qed.
+
+  Lemma listzzs_eqb_affine_product_eq :
+    forall affs1 affs2 p,
+      listzzs_eqb affs1 affs2 = true ->
+      affine_product affs1 p = affine_product affs2 p.
+  Proof.
+    induction affs1 as [|[v1 c1] affs1 IH]; intros [|[v2 c2] affs2] p Heq; simpl in *; try discriminate; auto.
+    apply andb_true_iff in Heq as [Hlen Hfor].
+    apply Nat.eqb_eq in Hlen. inversion Hlen. subst.
+    apply andb_true_iff in Hfor as [Hhead Htail].
+    apply andb_true_iff in Hhead as [Hv Hc].
+    apply Z.eqb_eq in Hc. simpl. f_equal.
+    - rewrite Hc. f_equal. apply dot_product_eq_compat_left. exact Hv.
+    - apply IH. apply andb_true_iff. split.
+      + apply Nat.eqb_eq. assumption.
+      + exact Htail.
+  Qed.
+
+  Lemma access_eqb_cell_eq : forall a1 a2 p,
+    access_eqb a1 a2 = true ->
+    cell_eq (exact_cell a2 p) (exact_cell a1 p).
+  Proof.
+    intros [id1 affs1] [id2 affs2] p Heq. simpl in *.
+    apply andb_true_iff in Heq as [Hid Haff].
+    apply Pos.eqb_eq in Hid. split; auto.
+    pose proof (listzzs_eqb_affine_product_eq affs1 affs2 p Haff) as Heval.
+    rewrite <- Heval. apply veq_refl.
+  Qed.
+
   Definition waccess (i : t) : option (list AccessFunction) :=
     match i with
     | SSkip => Some []
@@ -207,45 +376,9 @@ Module SInstr <: INSTR.
     | SAssign lhs _ => negb (existsb (ident_eqb (access_ident lhs)) ctxt)
     end.
 
-  Definition normalize_affine_rev (cols : nat) (aff : list Z * Z) : (list Z * Z) :=
-    let '(v, c) := aff in
-    (rev (resize cols v), c).
-
-  Definition normalize_affine_list_rev (cols : nat) (affs : list (list Z * Z)) :=
-    map (normalize_affine_rev cols) affs.
-
-  Definition normalize_affine (cols : nat) (aff : list Z * Z) : (list Z * Z) :=
-    let '(v, c) := aff in
-    (resize cols v, c).
-
-  Definition normalize_affine_list (cols : nat) (affs : list (list Z * Z)) :=
-    map (normalize_affine cols) affs.
-
-  Definition normalize_access (cols : nat) (acc : AccessFunction) : AccessFunction :=
-    let '(arrid, affs) := acc in
-    (arrid, normalize_affine_list cols affs).
-
-  Definition normalize_access_rev (cols : nat) (acc : AccessFunction) : AccessFunction :=
-    let '(arrid, affs) := acc in
-    (arrid, normalize_affine_list_rev cols affs).
-
-  Definition access_cols (acc : AccessFunction) : nat :=
-    let '(_, affs) := acc in
-    list_max (map (fun aff => let '(zs, _) := aff in length zs) affs).
-
   Definition access_function_checker_access
       (al : list AccessFunction) (a : access) : bool :=
-    let acc := access_to_function a in
-    existsb
-      (fun target =>
-        access_strict_eqb acc target ||
-        access_strict_eqb
-          (normalize_access (access_cols target) acc)
-          target ||
-        access_strict_eqb
-          (normalize_access_rev (access_cols target) acc)
-          target)
-      al.
+    existsb (fun target => access_eqb (access_to_function a) target) al.
 
   Fixpoint access_function_checker_expr
       (rl : list AccessFunction) (e : expr) : bool :=
@@ -270,14 +403,94 @@ Module SInstr <: INSTR.
         access_function_checker_expr rl rhs
     end.
 
+  Lemma access_function_checker_access_correct :
+    forall al a p,
+      access_function_checker_access al a = true ->
+      valid_access_cells p [access_cell a p] al.
+  Proof.
+    intros al a p Hchk. unfold access_function_checker_access in Hchk.
+    unfold valid_access_cells. intros c Hin. simpl in Hin. destruct Hin as [Heq|[]]. subst c.
+    apply existsb_exists in Hchk. destruct Hchk as [target [Hin Hacc]].
+    exists target. split; auto. apply access_eqb_cell_eq. exact Hacc.
+  Qed.
+
+  Lemma access_function_checker_expr_correct :
+    forall rl e p,
+      access_function_checker_expr rl e = true ->
+      valid_access_cells p (read_cells_expr e p) rl.
+  Proof.
+    induction e; intros p Hchk; simpl in *.
+    - apply valid_access_cells_nil.
+    - apply valid_access_cells_nil.
+    - apply access_function_checker_access_correct; exact Hchk.
+    - apply andb_true_iff in Hchk as [H1 H2].
+      eapply valid_access_cells_app; [apply IHe1|apply IHe2]; eauto.
+    - apply andb_true_iff in Hchk as [H1 H2].
+      eapply valid_access_cells_app; [apply IHe1|apply IHe2]; eauto.
+    - apply andb_true_iff in Hchk as [H1 H2].
+      eapply valid_access_cells_app; [apply IHe1|apply IHe2]; eauto.
+  Qed.
+
   Lemma access_function_checker_correct :
     forall wl rl i,
       access_function_checker wl rl i = true ->
       valid_access_function wl rl i.
   Proof.
-    intros wl rl i _. unfold valid_access_function. intros.
-    inversion H.
+    intros wl rl i Hchk p st st' wcells rcells Hsem.
+    inversion Hsem; subst; simpl in *.
+    - split; apply valid_access_cells_nil.
+    - apply andb_true_iff in Hchk as [Hwl Hrl].
+      split.
+      + apply access_function_checker_access_correct. exact Hwl.
+      + apply access_function_checker_expr_correct. exact Hrl.
   Qed.
+
+  Lemma eval_expr_write_irrelevant : forall e p st cell val,
+    Forall (fun rc => cell_neq rc cell) (read_cells_expr e p) ->
+    eval_expr e p (state_write st cell val) = eval_expr e p st.
+  Proof.
+    induction e; intros p st cell val Hneq; simpl in *; auto.
+    - inversion Hneq as [|? ? Hc _].
+      rewrite state_write_other; auto.
+    - apply Forall_app in Hneq as [H1 H2].
+      rewrite IHe1 by exact H1. rewrite IHe2 by exact H2. reflexivity.
+    - apply Forall_app in Hneq as [H1 H2].
+      rewrite IHe1 by exact H1. rewrite IHe2 by exact H2. reflexivity.
+    - apply Forall_app in Hneq as [H1 H2].
+      rewrite IHe1 by exact H1. rewrite IHe2 by exact H2. reflexivity.
+  Qed.
+
+  Lemma instr_semantics_stable_under_state_eq :
+    forall i p wcs rcs st1 st2 st1' st2',
+      State.eq st1 st1' ->
+      State.eq st2 st2' ->
+      instr_semantics i p wcs rcs st1 st2 ->
+      instr_semantics i p wcs rcs st1' st2'.
+  Proof.
+    intros i p wcs rcs st1 st2 st1' st2' Heq1 Heq2 Hsem.
+    destruct Hsem as
+        [p0 st10 st20 Heqskip
+        | lhs rhs p0 st10 st20 cell val Hcell Hval Hstate].
+    - econstructor.
+      eapply State.eq_trans.
+      + apply State.eq_sym. exact Heq2.
+      + eapply State.eq_trans; [exact Heqskip|exact Heq1].
+    - subst cell val. econstructor.
+      + reflexivity.
+      + symmetry. apply eval_expr_state_eq. apply State.eq_sym. exact Heq1.
+      + eapply State.eq_trans.
+        * apply State.eq_sym. exact Heq2.
+        * eapply State.eq_trans.
+          -- exact Hstate.
+          -- apply state_write_proper. exact Heq1.
+  Qed.
+
+  Lemma sema_prsv_nonalias :
+    forall i p wcs rcs st1 st2,
+      NonAlias st1 ->
+      instr_semantics i p wcs rcs st1 st2 ->
+      NonAlias st2.
+  Proof. intros; exact I. Qed.
 
   Definition is_iterator_varname (name : varname) : bool :=
     match name with
@@ -337,6 +550,72 @@ Module SInstr <: INSTR.
         instr_semantics i1 p1 wcs1 rcs1 st2' st3' /\
         State.eq st3 st3'.
   Proof.
-    intros. destruct H0 as [H12 _]. inversion H12.
+    intros i1 p1 wcs1 rcs1 st1 st2 st3 i2 p2 wcs2 rcs2 _ [Hsem1 Hsem2] [Hww [Hwr Hrw]].
+    destruct Hsem1 as
+        [p1' st10 st20 Heq12
+        | lhs1 rhs1 p1' st10 st20 cell1 val1 Hcell1 Hval1 Hstate1];
+    destruct Hsem2 as
+        [p2' st21 st30 Heq23
+        | lhs2 rhs2 p2' st21 st30 cell2 val2 Hcell2 Hval2 Hstate2].
+    - exists st10, st10.
+      split.
+      + constructor. apply State.eq_refl.
+      + split.
+        * constructor. apply State.eq_refl.
+        * eapply State.eq_trans; eauto.
+    - exists st30, st30.
+      split.
+      + eapply SemaAssign with (cell := cell2) (val := val2).
+        * exact Hcell2.
+        * rewrite Hval2. apply eval_expr_state_eq. exact Heq12.
+        * eapply State.eq_trans; [exact Hstate2|].
+          apply state_write_proper. exact Heq12.
+      + split.
+        * constructor. apply State.eq_refl.
+        * apply State.eq_refl.
+    - exists st10, st21.
+      split.
+      + constructor. apply State.eq_refl.
+      + split.
+        * eapply SemaAssign with (cell := cell1) (val := val1); eauto.
+        * exact Heq23.
+    - assert (Hneq12 : cell_neq cell1 cell2).
+      {
+        inversion Hww as [| ? ? Hcell _]; subst.
+        inversion Hcell as [| ? ? Hneq _]; subst.
+        exact Hneq.
+      }
+      assert (Hrhs2 : Forall (fun rc => cell_neq rc cell1) (read_cells_expr rhs2 p2')).
+      {
+        induction Hwr as [|rc rcs Hhead Htail IH]; constructor.
+        - inversion Hhead as [| ? ? Hneq _]; subst.
+          rewrite cell_neq_symm. exact Hneq.
+        - exact IH.
+      }
+      assert (Hrhs1 : Forall (fun rc => cell_neq rc cell2) (read_cells_expr rhs1 p1')).
+      {
+        inversion Hrw as [| ? ? Hhead _]; subst.
+        exact Hhead.
+      }
+      exists (state_write st10 cell2 val2),
+             (state_write (state_write st10 cell2 val2) cell1 val1).
+      split.
+      + eapply SemaAssign with (cell := cell2) (val := val2).
+        * exact Hcell2.
+        * rewrite Hval2.
+          rewrite (eval_expr_state_eq rhs2 p2' st21 (state_write st10 cell1 val1) Hstate1).
+          apply eval_expr_write_irrelevant. exact Hrhs2.
+        * apply State.eq_refl.
+      + split.
+        * eapply SemaAssign with (cell := cell1) (val := val1).
+          -- exact Hcell1.
+          -- rewrite Hval1.
+             symmetry. apply eval_expr_write_irrelevant. exact Hrhs1.
+          -- apply State.eq_refl.
+        * eapply State.eq_trans.
+          -- exact Hstate2.
+          -- eapply State.eq_trans.
+             ++ apply state_write_proper. exact Hstate1.
+             ++ apply state_write_commute. exact Hneq12.
   Qed.
 End SInstr.
